@prefix dash: <http://datashapes.org/dash#> .
@prefix rdf: <http://www.w3.org/1999/02/22-rdf-syntax-ns#> .
@prefix rdfs: <http://www.w3.org/2000/01/rdf-schema#> .
@prefix schema: <http://schema.org/> .
@prefix sh: <http://www.w3.org/ns/shacl#> .
@prefix xsd: <http://www.w3.org/2001/XMLSchema#> .
@prefix dct: <http://purl.org/dc/terms/> .
@prefix sosa: <http://www.w3.org/ns/sosa/> .
@prefix sam: <http://def.seegrid.csiro.au/ontology/sam-lite#> .
@prefix skos:  <http://www.w3.org/2004/02/skos/core#> .
@prefix gsqs: <http://linked.data.qld.gov.au/def/samples/> .


# gsqs:SimpleLithologyShape
#     a sh:NodeShape ;
#     sh:property [
#         # any SimpleLithologyShape Concept must have the property skos:inScheme once and only once
#         sh:path skos:inScheme;
#         sh:minCount 1 ;
#         sh:maxCount 1 ;
#         # that skos:inScheme property must have the value <http://resource.geosciml.org/classifierscheme/cgi/2016.01/simplelithology> (the Simple Lithology Concept Scheme URI)
#         sh:hasValue <http://resource.geosciml.org/classifierscheme/cgi/2016.01/simplelithology>
#     ] .

gsqs:SampleShape
    a sh:NodeShape ;
    sh:targetClass sosa:Sample;
    sh:property [
        sh:path sam:currentLocation ;
        sh:datatype xsd:string ;
        sh:name "current location" ;
        sh:minCount 1 ;
        sh:maxCount 1 ;
        rdfs:comment "Must have one and only one property sam:currentLocation indicating a string Literal object instance"
    ] ;
    sh:property [
        sh:path dct:accessRights;
        sh:in (
          "public"
          "private"
        ) ;
        sh:maxCount 1 ;
        rdfs:comment "Must have either 0 or 1 dct:accessRights properties which, if it exists, must indicate a string Literal object instance, one of 'public', 'private'"
    ] ;
    sh:property [
        sh:path sosa:isSampleOf;
        sh:minCount 1 ;
        sh:maxCount 1 ;
        sh:node gsqs:SiteShape;
        rdfs:comment "Must have one and only one property sosa:isSampleOf indicating a valid gsqs:SiteShape object"
    ] ;
    # must have one and only one sam:currentLocation that is a string Literal
    sh:property [
        sh:path gsqs:hasLithology;
        sh:minCount 1 ;
        sh:maxCount 1 ;
        sh:nodeKind sh:IRI ;
        rdfs:comment "Must have one and only property gsqs:hasLithology indicating a skos:Concept object instance that must be an IRI, i.e. not a Blank Node, and, in turn, has one and only one skos:inScheme properties indicating the skos:ConceptScheme instance <http://resource.geosciml.org/classifierscheme/cgi/2016.01/simplelithology>" ;
        sh:property [
            sh:path skos:inScheme ;
            sh:minCount 1 ;
            sh:maxCount 1 ;
            sh:hasValue <http://resource.geosciml.org/classifierscheme/cgi/2016.01/simplelithology>
        ]
    ] .
